twophase: prove list/slice conversion functions

src/goose_lang/lib/list/list_slice.v
@@ -7,20 +7,28 @@ Context `{ffi_sem: ext_semantics}.
 Context {ext_ty:ext_types ext}.
 Local Coercion Var' (s:string) : expr := Var s.
 
+Definition SliceToListFrom t : val :=
+  rec: "loop" "s" "i" :=
+    let: "len" := slice.len "s" in
+    if: ("i" < "len") then
+      let: "x" := SliceGet t "s" "i" in
+      ListCons "x" ("loop" "s" ("i" + #1))
+    else ListNilV.
+
 Definition SliceToList t : val :=
   λ: "s",
-  let: "len" := slice.len "s" in
-  (rec: "loop" "i" :=
-       if: ("i" < "len") then
-         let: "x" := SliceGet t "s" "i" in
-         ListCons "x" ("loop" ("i" + #1))
-       else ListNilV) #0.
+    SliceToListFrom t "s" #0%nat.
+
+Definition ListToSliceApp t : val :=
+  rec: "loop" "l" "s" :=
+    ListMatch "l"
+      (λ: "x", "s")
+      (λ: "p",
+        "loop" (Snd "p") (SliceAppend t "s" (Fst "p"))
+      ).
 
 Definition ListToSlice t : val :=
   λ: "l",
-  (rec: "loop" "l" "s" :=
-     ListMatch "l"
-               (λ: "x", "s")
-               (λ: "p", "loop" (Snd "p") (SliceAppend t "s" (Fst "p")))).
+    ListToSliceApp t "l" (NewSlice t #0).
 
 End goose_lang.
